presentation

theories/AllDifferent.v
@@ -4,7 +4,9 @@ Require Import Checker.Variable.
 Require Import Coq.NArith.NArith.
 Require Import Coq.ZArith.ZArith.
 Require Import Coq.Lists.List.
+Require Import Lia.
 Import Utility.Sets.
+Import Utility.ListEx.
 
 Module Z_String_as_OT := OrdersEx.PairOrderedType OrdersEx.Z_as_OT OrdersEx.String_as_OT.
 Module sintstr := MSetAVL.Make Z_String_as_OT.
@@ -41,11 +43,11 @@ Definition valuation_from_assignment (c : AllDifferentConstraint) (a : Assignmen
     end
   .
 
-Definition AllDifferent (c : sstr.t) (v : string -> Z) : Prop :=
-  (forall (x y : string), 
-  x <> y -> sstr.In x c -> sstr.In y c -> v x <> v y).
+Definition AllDifferent (vs : list string) (v : string -> Z) : Prop :=
+  forall x y, 
+  x <> y -> In x vs -> In y vs -> v x <> v y.
 
-Definition find_conflict_filter_f (n : Z) (el: (Z * string)) :=
+(* Definition find_conflict_filter_f (n : Z) (el: (Z * string)) :=
   let (n', _) := el in (n =? n')%Z.
 
 Definition find_conflict (x : string) (n : Z) (values : sintstr.t) : option (Z * string) := 
@@ -79,7 +81,7 @@ Definition alldifferent_decide (constraint : AllDifferentConstraint) (a : Assign
   let valuation := valuation_from_assignment constraint a in
   dec_all_different constraint.(vars_ad) valuation
 .
-
+ *)
 (* Definition AllDifferent (c : sstr.t) (v : string -> Z) : Prop :=
   (forall (x y : string), 
   x <> y -> sstr.In x c -> sstr.In y c -> v x <> v y).
@@ -101,7 +103,7 @@ Definition state := string -> FullDomain.
 Definition dom_size (dom : BoundedDomain) : Z :=
   dom.(bd_ub) - dom.(bd_lb) + 1 - (Z.of_nat (sint.cardinal dom.(bd_holes))).
  *)
-Definition dom_size (dom : FullDomain) : nat := sint.cardinal dom.
+(* Definition dom_size (dom : FullDomain) : nat := sint.cardinal dom. *)
 
 Definition vars_dom_union (st : state) (vs : sstr.t) := 
     sstr.fold 
@@ -110,47 +112,358 @@ Definition vars_dom_union (st : state) (vs : sstr.t) :=
     sint.empty.
 
 Definition vars_len (vs : sstr.t) : nat := sstr.cardinal vs.
-
+ 
 Open Scope nat_scope.
 
-Definition ex_confl_set (st : state) (vs : sstr.t) := 
+(* Definition ex_confl_set (st : state) (vs : sstr.t) := 
   exists confl_vars, 
     sstr.Subset confl_vars vs 
       /\ 
     dom_size (vars_dom_union st confl_vars) < vars_len confl_vars.
+ *)
 
-Definition valuation_in_state (st : state) (vs : sstr.t) (v : string -> Z) : Prop :=
-  forall (x : string), sstr.In x vs -> sint.In (v x) (st x).
+Definition valuation_in_state (st : state) (vs : list string) (v : string -> Z) : Prop :=
+  forall x, In x vs -> sint.In (v x) (st x).
 
-Definition AllDifferent_sat (st : state) (vs : sstr.t) :=
-  exists v, valuation_in_state st vs v -> AllDifferent vs v.
+Definition AllDifferent_sat (st : state) (vs : list string) :=
+  exists v, valuation_in_state st vs v /\ AllDifferent vs v.
 
-Lemma conflict_if_ex_confl_set (st : state) (vs : sstr.t) :
-  ex_confl_set st vs -> ~ AllDifferent_sat st vs.
+(* Lemma all_different_subset (v : string -> Z) :
+  forall (vs : sstr.t) (vs' : sstr.t),
+  AllDifferent vs v -> sstr.Subset vs' vs -> AllDifferent vs' v.
 Proof.
-  intros H.
-  destruct H as [confl_vars [Hsub Hlt]].
-  unfold AllDifferent_sat. intros Halldiff.
-  destruct Halldiff as [v [Hdom Hdiff]].
-  enough (dom_size (vars_union_domain st confl_vars) >= vars_len confl_vars).
-  - apply Nat.lt_nge in Hlt.
-    contradiction.
-  - apply all_different_subset with (vs' := confl_vars) in Hdiff; try assumption.
-    destruct (alldiff_valuation_values_props confl_vars st v Hdiff) as [Hvals Hins].
-    rewrite Hvals.
-    unfold ge.
-    apply sint_prps.subset_cardinal.
-    unfold sint.Subset.
-    intros n Hin.
-    destruct (Hins n Hin)  as [x [Hxin Hvx]].
-    subst n.
-    specialize (vars_union_domain_correct st confl_vars x Hxin) as Hunion.
+  intros vs vs'. intros Hdiff Hsub.
+  unfold AllDifferent in *.
+  intros x y.
+  intros Hxny Hinx Hiny.
+  apply Hdiff; try assumption; apply Hsub; assumption.
+Qed.
+ *)
+(* Lemma alldiff_valuation_values_props (c : sstr.t) (st : state) :
+  forall (v: string -> Z), AllDifferent c v 
+    -> 
+  vars_len c = sint.cardinal (valuation_values c v) 
+    /\ 
+  forall n, sint.In n (valuation_values c v) -> exists x, sstr.In x c /\ v x = n.
+Proof.
+Admitted. *)
+  (* intros v Hval_alldiff. unfold AllDifferent in Hval_alldiff.
+  unfold valuation_values.
+  set (P := 
+      fun (s : sstr.t) (acc : sint.t) =>
+      vars_len s = sint.cardinal acc 
+      /\ forall n, sint.In n acc -> exists x, sstr.In x s /\ sstr.In x c /\ v x = n
+  ).
+  enough (P c (sstr.fold (valuation_values_foldf v) c
+  sint.empty)).
+  { 
+    unfold P in H. clear P. destruct H as [Hcard Hn].
+    repeat split; try assumption.
+    intros n Hin. destruct (Hn n Hin) as [x [Hinc [_ Hvx]]].
+    exists x. split; try assumption.
+  }
+  apply sstr_prps.fold_rec with (f := valuation_values_foldf v) (i := sint.empty) (s := c) (P := P).
+  - autounfold with short_unfold_db in *.
+    unfold P in *. clear P. intros s Hempty.
+    repeat split.
+    + unfold vars_len. rewrite sint.cardinal_spec. simpl. rewrite sstr_prps.cardinal_Empty in Hempty. rewrite Hempty. reflexivity. 
+    + intros n Hinempty.
+      exfalso.
+      apply (sint.empty_spec Hinempty).
+  - intros var vals s s_v.
+    intros Hin Hvarnots Hadd IH.
+    unfold P in *. clear P.
     autounfold with short_unfold_db in *.
-    apply Hunion.
-    apply Hdom.
-    apply Hsub.
-    exact Hxin.
+    destruct IH as [IH_card Hinvar].
+    repeat split.
+    + unfold vars_len.
+      rewrite sstr_prps.Add_Equal in Hadd.
+      apply sstr_prps.Equal_cardinal in Hadd.
+      rewrite Hadd.
+      unfold valuation_values_foldf.
+      rewrite (sstr_prps.add_cardinal_2 Hvarnots).
+      assert (~ sint.In (v var) vals) as Hvvarnotvals.
+      { 
+        intros Hvvarin.
+        destruct (Hinvar (v var) Hvvarin) as [x [Hxins [Hxinc Hvx]]].
+        apply Hval_alldiff with (x := var) (y := x); try assumption.
+        + intros Hvarisx. apply Hvarnots. rewrite Hvarisx. exact Hxins.
+        + symmetry. assumption.
+      }
+      rewrite (sint_prps.add_cardinal_2 Hvvarnotvals).
+      f_equal.
+      exact IH_card.        
+    + intros n Hinfoldf.
+      unfold valuation_values_foldf in Hinfoldf.
+      rewrite sint.add_spec in Hinfoldf.
+      destruct Hinfoldf as [Hvvar | Hnvals].
+      * exists var.
+        repeat split.
+        { apply Hadd. left. reflexivity. }
+        { exact Hin. }
+        { symmetry. exact Hvvar. }
+      * specialize (Hinvar n Hnvals).
+        destruct Hinvar as [x [Hxins [Hxinc Hvx]]].
+        exists x.
+        repeat split; try assumption.
+        apply Hadd.
+        right. assumption.
+Qed. *)
+
+(* Lemma AllDifferent_elements (vs : sstr.t) (v : string -> Z) :
+  AllDifferent vs v
+    ->
+  (forall (x y : string), 
+  x <> y -> In x (sstr.elements vs) -> In y (sstr.elements vs) -> v x <> v y).
+Proof.
+  intros Hdiff x y Hxny Hinx Hiny.
+  specialize (Hdiff x y Hxny).
+  apply Hdiff; now apply sstr.elements_spec_in.
+Qed. 
+ *)
+Lemma sint_cardinal_union_diff :
+  forall s s', sint.cardinal (sint.union s s') = sint.cardinal (sint.diff s s') + sint.cardinal s'.
+Proof.
+  intros s s'.
+  rewrite sint_prps.union_cardinal_inter.
+  rewrite <- sint_prps.diff_inter_cardinal with (s := s) (s' := s'). lia.
 Qed.
 
+Ltac solve_disjunction :=
+  first
+    [ assumption
+    | reflexivity
+    | match goal with
+      | |- _ \/ _ =>
+          (left; solve_disjunction)
+          ||
+          (right; solve_disjunction)
+      end
+    ].
+
+Ltac break_in_hyps :=
+  repeat match goal with
+  | [ H: In ?x _  |- In ?x _ ] => simpl in H
+  end;
+  repeat match goal with
+  | [ H: _ \/ In ?x _ |- In ?x _ ] =>
+      let Hnew := fresh H in
+      destruct H as [Hnew | Hnew]; subst; try discriminate
+  end;
+  simpl.
+
+Ltac solve_in := break_in_hyps; try solve_disjunction.
+
+(* Definition is_domain_union (st : state) (vars : list string) (union : list Z) :=
+  NoDup union
+    /\
+  forall n, In n union <-> (exists x, In x vars /\ sint.In n (st x)).
+
+Definition ex_confl_vars (st : state) (vs : list string) := 
+  exists confl_vars union,
+    NoDup confl_vars
+      /\
+    incl confl_vars vs
+      /\ 
+    is_domain_union st confl_vars union
+      /\ 
+    length union < length confl_vars.
+ *)
+
+Definition is_domain_union (st : state) (variables : list string) (domain_union : list Z) :=
+  NoDup domain_union
+    /\
+  forall n, In n domain_union <-> (exists x, In x variables /\ sint.In n (st x)).
+
+Definition exists_conflict_variables (st : state) (constraint_variables : list string) := 
+  exists conflict_variables conflict_domain_union,
+    NoDup conflict_variables
+      /\
+    incl conflict_variables constraint_variables
+      /\ 
+    is_domain_union st conflict_variables conflict_domain_union
+      /\ 
+    length conflict_domain_union < length conflict_variables.
+
+
+Import Datatypes.
+
+Lemma conflict_if_ex_confl_vars (st : state) (constraint_variables : list string) :
+  exists_conflict_variables st constraint_variables -> ~ AllDifferent_sat st constraint_variables.
+Proof.
+  intros (conflict_variables & conflict_domain_union & Hnodup & Hsub & Hunion & Hlengths).
+  intros [A [Hastate Halldiff]].
+  enough (length conflict_domain_union >= length conflict_variables).
+  { apply Nat.lt_nge in Hlengths.
+    contradiction. }
+  clear Hlengths; rewrite <- length_map with (f := A).
+  apply NoDup_incl_length.
+  - clear -Hnodup Halldiff Hsub. 
+    apply Injective_map_NoDup_in.
+    * intros x y Hinx Hiny Hvxvy.
+      destruct (String.string_dec x y) as [Hxy | Hxy].
+      { assumption. }
+      enough (A x <> A y) by contradiction.
+      apply Halldiff; try apply Hsub; assumption.
+    * apply Hnodup.
+  - clear -Hunion Hastate Hsub. 
+    unfold incl. intros n Hin. 
+    apply Hunion; clear Hunion.
+    rewrite in_map_iff in Hin.
+    destruct Hin as (x & Hvx & Hxin).
+    exists x. split.
+    + exact Hxin.
+    + rewrite <- Hvx. apply Hastate.
+      apply Hsub. exact Hxin.
+Qed.
+(* destruct H as (conflict_variables & union & Hnodup & Hsub & Hunion & Hlt).
+  intros [v [Hvstate Hdiff]].
+  enough (length union >= length confl_vars).
+  { apply Nat.lt_nge in Hlt.
+    contradiction. } 
+  rewrite <- length_map with (f := v).
+  apply NoDup_incl_length.
+  - apply Injective_map_NoDup_in.
+    * intros x y Hinx Hiny Hvxvy.
+      destruct (String.string_dec x y) as [Hxy | Hxy].
+      { assumption. }
+      enough (v x <> v y) by contradiction.
+      apply Hdiff; try apply Hsub; assumption.
+    * apply Hnodup.
+  - unfold incl. destruct Hunion as [Hunion_nodup Hunion].
+    intros n Hin.
+    rewrite in_map_iff in Hin.
+    destruct Hin as (x & Hvx & Hxin).
+    rewrite (Hunion n).
+    exists x. split.
+    + exact Hxin.
+    + rewrite <- Hvx. apply Hvstate.
+      apply Hsub. exact Hxin.
+Qed.
+ *)
+
+Lemma computed_confl (st : state) :
+  forall confl_vars vs,
+    sstr.Subset confl_vars vs
+      ->
+    sint.cardinal (vars_dom_union st confl_vars) < sstr.cardinal confl_vars
+      ->
+    exists_conflict_variables st (sstr.elements vs).
+Proof.
+  intros confl_vars vs.
+  intros Hsub Hlt.
+  unfold exists_conflict_variables.
+  exists (sstr.elements confl_vars).
+  exists (sint.elements (vars_dom_union st confl_vars)). 
+  split; [|split]; [| |split].
+  - apply sstr.elements_spec_nodup.
+  - intros x. repeat rewrite sstr.elements_spec_in.
+    apply Hsub.
+  - split.
+    { apply sint.elements_spec_nodup. }
+    unfold vars_dom_union.
+    rewrite sstr.fold_spec.
+    rewrite <- fold_left_rev_right.
+    setoid_rewrite in_rev at 2.
+    rename confl_vars into confl_vars'.
+    remember (rev (sstr.elements confl_vars')) as vl.
+    setoid_rewrite <- Heqvl.
+    clear.
+    setoid_rewrite sint.elements_spec_in.
+    induction vl as [|v vl IH].
+    + simpl. intros n.
+      split; intros H.
+      * exfalso. apply (sint.empty_spec H).
+      * destruct H as (Hx & Hf & _). contradiction.
+    + intros n.
+      simpl.
+      rewrite sint.union_spec.
+      rewrite (IH n). clear.
+      split; intros H.
+      * destruct H.
+        -- exists v. split; solve_disjunction.
+        -- destruct H as (x & Hinvl & Hinst).
+          exists x. split; solve_disjunction.
+      * destruct H as (x & Hvx & Hinst).
+        destruct Hvx.
+        -- subst x. now left.
+        -- right. exists x. now split.
+  - rewrite <- sint.cardinal_spec. rewrite <- sstr.cardinal_spec.
+    apply Hlt.
+Qed. 
+
+    
+
+
+(*     
+
+
+  induction l.
+  - simpl. lia.
+  - simpl. 
+    rewrite sint_cardinal_union_diff.
+    remember (fold_right
+      (fun (y : sstr.elt) (x : sint.t)
+      => sint.union (st y) x)
+      sint.empty l) as s.
+    assert (sint.cardinal s >= length l) as Hlen.
+    { apply IHl.
+      - intros. apply Hdiff_l; simpl; try right; assumption.
+      - intros. apply Hlstate. right; assumption.
+      - inversion Hnodup; assumption. }
+    clear IHl.
+    enough (sint.cardinal (sint.diff (st a) s) >= 1) by lia.
+    enough (In (v a) (sint.elements (sint.diff (st a) s))).
+    { rewrite sint.cardinal_spec. destruct sint.elements; simpl; try lia. destruct H. }
+    rewrite sint.elements_spec_in.
+    rewrite sint.diff_spec.
+    split.
+    { apply Hlstate. left. reflexivity. }
+    subst s; clear Hlen. induction l as [|a' l IH].
+    + simpl. intros Hin. apply (sint.empty_spec Hin).
+    + simpl. rewrite sint.union_spec.
+      intros [Hva' | Hfold].
+      * clear IH.
+        admit.  
+      * apply IH; try assumption.
+        -- intros. apply Hdiff_l.
+          ++ assumption.
+          ++ solve_in.
+          ++ solve_in.
+        -- intros. apply Hlstate.
+          solve_in.
+        -- inversion Hnodup; subst.
+          inversion H2; subst.
+          apply NoDup_cons.
+          ++ intros Hin. apply H1.
+            solve_in.
+          ++ assumption.
+Qed.
+
+
+      - intros. apply Hlstate. right; assumption.
+      - inversion Hnodup; assumption. }
+
+    enough (length (sint.elements (sint.union (st a) s)) >= S (length (sint.elements s))) by lia; clear Hlen.
+    enough (~ In (v a) (sint.elements s) /\ In (v a) (sint.elements (sint.union (st a) s))).
+    {  }
+    
+    rewrite fold_right_app.
+  destruct (alldiff_valuation_values_props confl_vars st v Hdiff) as [Hvals Hins].
+  rewrite Hvals.
+  unfold ge.
+  apply sint_prps.subset_cardinal.
+  unfold sint.Subset.
+  intros n Hin.
+  destruct (Hins n Hin)  as [x [Hxin Hvx]].
+  subst n.
+  specialize (vars_union_domain_correct st confl_vars x Hxin) as Hunion.
+  autounfold with short_unfold_db in *.
+  apply Hunion.
+  apply Hdom.
+  apply Hsub.
+  exact Hxin.
+Qed.
+ *)
 (* Definition ex_confl_set (st : state) (vs : vars) := 
 (exists (confl_vars : vars), sstr.Subset confl_vars vs /\ dom_size (vars_union_domain st confl_vars) < vars_len confl_vars). *)
